Reorganize; clean up interfaces in extension.v

veric/extension.v
@@ -158,21 +158,22 @@ Module Extension. Section Extension.
      (exists rv, safely_halted CS ge c = Some rv) \/
      (exists ef, exists sig, exists args, at_external CS c = Some (ef, sig, args));
 
- (** A core is no longer "at external" once the extension has returned 
-    to it with the result of the call on which it was blocked. *)
-   after_at_external_excl : forall i CS c c' ret,
-     csem i = Some CS -> after_external CS ret c = Some c' -> 
-     at_external CS c' = None;
-   
+ (** AtExternal cores are blocked on external functions specified by their
+    external function signatures. *)
    at_external_csig: forall s i CS c ef args sig,
      csem i = Some CS -> proj_core i s = Some c -> 
      at_external CS c = Some (ef, sig, args) -> 
      IN ef csig;
+
+ (** When a core is AtExternal but the extension is not, the function on which 
+    the core is blocked is handled by the extension. *)
    notat_external_handled: forall s i CS c ef args sig,
      csem i = Some CS -> proj_core i s = Some c -> 
      at_external CS c = Some (ef, sig, args) -> 
      at_external esem s = None -> 
      IN ef handled;
+
+ (** Functions on which the extension is blocked are not handled. *)
    at_external_not_handled: forall s ef args sig,
      at_external esem s = Some (ef, sig, args) -> 
      NOTIN ef handled;
@@ -199,7 +200,7 @@ Implicit Arguments Extension.Make [G xT cT M D Z Zint Zext].
 
 (** * Safe Extensions *)
 
-Section AllSafety.
+Section SafeExtension.
  Variables
   (G: Type) (** global environments *)
   (xT: Type) (** corestates of extended semantics *)
@@ -231,7 +232,7 @@ Definition safe_extension (E: Sig cT Zint esem csem csig esig handled) :=
     all_safe E ge n (zmult E (proj_zint E s) z) s m -> 
     safeN esem (link esig handled) ge n z s m.
 
-End AllSafety.
+End SafeExtension.
 
 Module SafetyInvariant. Section SafetyInvariant.
  Variables
@@ -270,7 +271,6 @@ Notation "'CORE' i 'is' ( CS , c ) 'in' s" :=
 Notation core_exists := E.(Extension.core_exists).
 Notation active_csem := E.(Extension.active_csem).
 Notation active_proj_core := E.(Extension.active_proj_core).
-Notation after_at_external_excl := E.(Extension.after_at_external_excl).
 Notation notat_external_handled := E.(Extension.notat_external_handled).
 Notation at_external_not_handled := E.(Extension.at_external_not_handled).
 Notation ext_upd_at_external := E.(Extension.ext_upd_at_external).
@@ -385,7 +385,7 @@ Inductive safety_invariant: Type := SafetyInvariant: forall
 
 End SafetyInvariant. End SafetyInvariant.
 
-Module EXTENSION_SOUNDNESS. Section EXTENSION_SOUNDNESS.
+Module EXTENSION_SAFETY. Section EXTENSION_SAFETY.
  Variables
   (G: Type) (** global environments *)
   (xT: Type) (** corestates of extended semantics *)
@@ -406,130 +406,154 @@ Module EXTENSION_SOUNDNESS. Section EXTENSION_SOUNDNESS.
 
 Import SafetyInvariant.
 
-Record Sig := Make {extension_sound: safety_invariant E -> safe_extension E}.
+Record Sig := Make {_: safety_invariant E -> safe_extension E}.
 
-End EXTENSION_SOUNDNESS. End EXTENSION_SOUNDNESS.
+End EXTENSION_SAFETY. End EXTENSION_SAFETY.
 
-(* Here we begin to develop a notion of compilable extension *)
-
-Lemma mem_unchanged_on_trans: 
-  forall P m m'' m',
-  mem_unchanged_on P m m'' -> 
-  mem_unchanged_on P m'' m' -> 
-  mem_unchanged_on P m m'.
-Proof.
-intros until m'; intros [H1 H2] [H3 H4].
-split.
-intros b ofs k p H5 H6 H7.
-specialize (H1 _ _ _ _ H5 H6 H7).
-eapply H3; eauto.
-eapply Mem.perm_valid_block; eauto.
-intros until v; intros H5 H6 H7.
-specialize (H2 _ _ _ _ H5 H6 H7).
-eapply H4; eauto.
-apply Mem.load_valid_access in H2.
-apply Mem.valid_access_implies with (p2 := Nonempty) in H2.
-eapply Mem.valid_access_valid_block; eauto.
-econstructor; eauto.
-Qed.
-
-Lemma mem_unchanged_on_weaken:
-  forall (P P': block -> Z -> Prop) m m',
-  (forall b ofs, P' b ofs -> P b ofs) -> 
-  mem_unchanged_on P m m' -> 
-  mem_unchanged_on P' m m'.
-Proof.
-intros until m'; intros H1 [H2 H3].
-split.
-intros until p; intros H4 H5 H6.
-solve[apply (H2 _ _ _ _ H4 (H1 _ _ H5) H6)].
-intros until v; intros H4 H5 H6.
-eapply H3; eauto.
-Qed.
+(**  "Compilable" Extensions *)
 
 (*This is an [F,V]-independent definition of meminj_preserves_globals*)
 Definition meminj_preserves_globals (globals: list block) f :=
   (forall b, In b globals -> f b = Some (b, 0)) /\
   (forall b1 b2 delta, In b2 globals -> f b1 = Some (b2, delta) -> b1=b2).
 
-Lemma meminj_preserves_globals_incr: 
-  forall globals f f' m1 m2,
-  inject_incr f f' -> 
-  inject_separated f f' m1 m2 -> 
-  Mem.inject f m1 m2 -> 
-  meminj_preserves_globals globals f -> 
-  meminj_preserves_globals globals f'.
-Proof.
-intros until m2; intros H1 SEP INJ [H2 H3].
-split.
-intros b H4.
-specialize (H2 _ H4).
-solve[eapply H1; eauto].
-intros until delta; intros H4 H5.
-specialize (H3 b1 b2 delta H4).
-case_eq (f b1).
-intros [b' ofs'] H6.
-specialize (H1 _ _ _ H6).
-rewrite H1 in H5; inv H5.
-apply H3; auto.
-intros H6.
-unfold inject_separated in SEP.
-destruct (SEP _ _ _ H6 H5) as [H7 H8].
-specialize (H2 _ H4).
-elimtype False.
-apply H8.
-apply (Mem.valid_block_inject_2 _ m1 _ _ _ _ H2); auto.
-Qed.
-
 Definition genv2blocks {F V: Type} (g: Genv.t F V) := 
   map snd (PTree.elements (Genv.genv_symb g)).
 
-Import Sim_inj.
+(** Some administrative requirements on the interactions between
+   extensions and inner cores. Perhaps some of these conditions could be 
+   merged with those for "safe" extensions. *)
 
-Module RGSimulationInject. Section RGSimulationInject.
+Section CoreCompatible.
+Variables 
+ (G xT M D Z Zint Zext: Type) (cT: nat -> Type)
+ (esem: CoreSemantics G xT M D) 
+ (csem: forall i:nat, option (CoreSemantics G (cT i) M D))
+ (csig: ext_sig M Z)
+ (esig: ext_sig M Zext)
+ (handled: list AST.external_function)
+ (E: Extension.Sig cT Zint esem csem csig esig handled).
+
+Import Extension.
+
+Inductive core_compatible: Type := CoreCompatible: forall
+  (** When the active thread is runnable, a step in the extended
+     semantics can be tracked back to a corestep of the active
+     thread. *)
+  (runnable_corestep: forall ge s m s' m' c CS,
+    runnable E ge s=true -> 
+    csem (active E s) = Some CS -> 
+    proj_core E (active E s) s = Some c -> 
+    corestep esem ge s m s' m' -> 
+    exists c', 
+      corestep CS ge c m c' m' /\ 
+      proj_core E (active E s) s' = Some c') 
+
+  (** After a corestep of the active inner core, the active thread's new
+     corestate is appropriately injected into the extended state. *)
+  (corestep_pres: forall ge s (c: cT (active E s)) m c' s' m' CS,
+    csem (active E s) = Some CS -> 
+    proj_core E (active E s) s = Some c -> 
+    corestep CS ge c m c' m' -> 
+    corestep esem ge s m s' m' -> 
+    active E s = active E s' /\ 
+    proj_core E (active E s) s' = Some c')
+  (** A corestep of the currently active core forces a corestep of the
+     extended semantics*)
+  (corestep_prog: forall ge s (c: cT (active E s)) m c' m' CS,
+    csem (active E s) = Some CS ->  
+    proj_core E (active E s) s = Some c -> 
+    corestep CS ge c m c' m' -> 
+    exists s', corestep esem ge s m s' m')
+
+  (** Other cores remain unchanged after coresteps of the active core. *)
+  (corestep_others_forward: forall ge s s' (c: cT (active E s')) m c' m' CS,
+    csem (active E s') = Some CS -> 
+    proj_core E (active E s') s' = Some c' -> 
+    corestep CS ge c m c' m' -> 
+    corestep esem ge s m s' m' -> 
+    forall j, (active E s)<>j -> proj_core E j s = proj_core E j s')
+  (corestep_others_backward: forall ge s c m s' c' m' CS n,
+    csem (active E s) = Some CS -> proj_core E (active E s) s = Some c -> 
+    corestepN CS ge n c m c' m' -> corestepN esem ge n s m s' m' -> 
+    forall j, (active E s)<>j -> proj_core E j s = proj_core E j s')
+
+  (** The active core doesn't change along active coresteps. *)
+  (after_ext_pres: forall s (c: cT (active E s)) c' s' CS retv,
+    csem (active E s) = Some CS -> 
+    proj_core E (active E s) s = Some c -> 
+    after_external CS retv c = Some c' -> 
+    after_external esem retv s = Some s' -> 
+    active E s=active E s')
+  (** The extension state can be updated to match AfterExternal on the 
+     active core. *)
+  (after_ext_prog: forall s (c: cT (active E s)) c' CS retv,
+    csem (active E s) = Some CS -> 
+    proj_core E (active E s) s = Some c -> 
+    after_external CS retv c = Some c' -> 
+    exists s', after_external esem retv s = Some s' /\
+      proj_core E (active E s) s' = Some c')
+
+  (** AfterExternal on extension cores leaves all but the active
+     corestate unchanged. *)
+  (after_ext_others: forall s s' retv,
+    after_external esem retv s = Some s' -> 
+    forall j, (active E s)<>j -> 
+      proj_core E j s = proj_core E j s')
+
+  (** REPEATED HERE TO GET AROUND A BUG IN PROGRAM: 
+     HYP (1) NOT GENERATED WHEN PROVING OBLIGATION *)
+  (at_extern_call: forall s ef sig args,
+    at_external esem s = Some (ef, sig, args) -> 
+    exists CS, exists c, 
+      csem (active E s) = Some CS /\ proj_core E (active E s) s = Some c /\
+      at_external CS c = Some (ef, sig, args)),
+  core_compatible.
+
+End CoreCompatible.
+
+(** Rely-Guarantee Simulations *)
+
+Module RelyGuaranteeSimulation. Section RelyGuaranteeSimulation.
  Variables (F1 V1 C1 INIT1 G2 C2 INIT2: Type).
  Variables 
   (sourceC: CoreSemantics (Genv.t F1 V1) C1 mem INIT1)
   (targetC: CoreSemantics G2 C2 mem INIT2) 
   (ge1: Genv.t F1 V1) (ge2: G2) 
   (entry_points: list (val * val * signature)).
+
+ Import Sim_inj.
+
  Variable (simC: Forward_simulation_inject _ _ sourceC targetC ge1 ge2 entry_points).
 
  Inductive Sig: Type := Make: forall
-  (RELY: forall (ge1: Genv.t F1 V1) cdC m1 m1' f f' m2 m2' c1 c2,
-    (*RELY*)
+  (rely: forall (ge1: Genv.t F1 V1) cdC m1 m1' f f' m2 m2' c1 c2,
+    (** Rely *)
     Mem.inject f m1 m2 -> 
     meminj_preserves_globals (genv2blocks ge1) f -> 
-
-    (* (*OTHER CORE DIAGRAM*) *)
-    (* match_state simD cdD f d1 m1 d2 m2 ->  *)
-    (* corestep sourceD ge1 d1 m1 d1' m1' ->  *)
-    (* corestepN  targetD ge2 n d2 m2 d2' m2' ->  *)
-    (* match_state simD cdD' f' d1' m1' d2' m2' ->  *)
-
-    (*OTHER CORE GUARANTEE*)
+    (** Plus other core guarantee*)
     Mem.inject f' m1' m2' -> 
     mem_unchanged_on (loc_unmapped f) m1 m1' ->
     mem_unchanged_on (loc_out_of_reach f m1) m2 m2' ->
     inject_incr f f' -> 
     inject_separated f f' m1 m2 -> 
 
-    (*THEN MATCH IS STABLE*)
+    (** Match is stable *)
     match_state simC cdC f c1 m1 c2 m2 -> 
     match_state simC cdC f' c1 m1' c2 m2')
     
-  (GUARANTEE: forall ge1 ge2 cd cd' m1 m1' f f' m2 m2' c1 c2 c1' c2' n,
-    (*RELY*)
+  (guarantee: forall ge1 ge2 cd cd' m1 m1' f f' m2 m2' c1 c2 c1' c2' n,
+    (** Rely *)
     Mem.inject f m1 m2 -> 
     meminj_preserves_globals (genv2blocks ge1) f -> 
 
-    (*DIAGRAM*)
+    (** Diagram *)
     match_state simC cd f c1 m1 c2 m2 -> 
     corestep sourceC ge1 c1 m1 c1' m1' -> 
     corestepN targetC ge2 n c2 m2 c2' m2' -> 
     match_state simC cd' f' c1' m1' c2' m2' -> 
 
-    (*GUARANTEE*)
+    (** Guarantee *)
     Mem.inject f' m1' m2' /\ 
     mem_unchanged_on (loc_unmapped f) m1 m1' /\
     mem_unchanged_on (loc_out_of_reach f m1) m2 m2' /\
@@ -537,163 +561,174 @@ Module RGSimulationInject. Section RGSimulationInject.
     inject_separated f f' m1 m2),
   Sig.
 
-End RGSimulationInject. End RGSimulationInject.
+End RelyGuaranteeSimulation. End RelyGuaranteeSimulation.
 
-(*STUFF AFTER THIS LINE CAN PROBABLY BE IGNORED*)
-Module CompilableSem. Section CompilableSem.
- Variables (F V: Type).
- Variable (sem: list block -> mem -> mem -> Prop).
-
- Inductive Sig: Type := Make: forall 
-   (PERM: forall ge m1 m1' b ofs p,
-     sem ge m1 m1' ->      
-     Mem.valid_block m1 b -> 
-     Mem.perm m1' b ofs Max p -> Mem.perm m1 b ofs Max p)
-   (VALID: forall ge m1 m1' b, 
-     sem ge m1 m1' -> 
-     Mem.valid_block m1 b -> Mem.valid_block m1' b)
-   (EXTENSIBLE: forall ge m1 m1' f m2,
-     meminj_preserves_globals ge f ->
-     sem ge m1 m1' -> 
-     Mem.extends m1 m2 ->
-     exists m2',
-       sem ge m2 m2' /\
-       Mem.extends m1' m2' /\
-       mem_unchanged_on (loc_out_of_bounds m1) m2 m2')
-   (INJECTIBLE: forall ge m1 m1' f m2,
-     meminj_preserves_globals ge f ->
-     sem ge m1 m1' -> 
-     Mem.inject f m1 m2 ->
-     exists f', exists m2',
-       sem ge m2 m2' /\
-       Mem.inject f' m1' m2' /\
-       mem_unchanged_on (loc_unmapped f) m1 m1' /\
-       mem_unchanged_on (loc_out_of_reach f m1) m2 m2' /\
-       inject_incr f f' /\
-       inject_separated f f' m1 m2),
-   Sig.
-
-End CompilableSem.
-
-Section CompilableTrans.
-Variables (sem1 sem2: list block -> mem -> mem -> Prop).
-
-Definition sem12 ge m1 m3 := exists m2, sem1 ge m1 m2 /\ sem2 ge m2 m3.
-
-Lemma compilable_trans: Sig sem1 -> Sig sem2 -> Sig sem12.
-Proof.
-intros H1 H2;
-destruct H1 as [PERM1 VALID1 EXT1 INJ1]; 
-destruct H2 as [PERM2 VALID2 EXT2 INJ2].
-constructor.
-(*PERM*)
-clear -VALID1 VALID2 PERM1 PERM2.
-intros until p; intros H1 H2.
-destruct H1 as [m1'' [SEM1 SEM2]]; eauto.
-(*VALID*)
-clear -VALID1 VALID2 PERM1 PERM2.
-intros until b; intros H1 H2.
-destruct H1 as [m1'' [SEM1 SEM2]]; eauto.
-(*EXTENSIBLE*)
-intros until m2; intros H1 H2 H3.
-destruct H2 as [m1'' [SEM1 SEM2]].
-exploit EXT1; eauto; intros [m2'' [H4 [H5 H6]]].
-exploit EXT2; eauto; intros [m2' [H7 [H8 H9]]].
-exists m2'; split. 
-exists m2''; split; auto.
-split; auto.
-generalize (@mem_unchanged_outofbounds_trans _ _ _ _ m2' 
- H3 H5 H6); intro H10.
-spec H10; eauto.
-(*INJECTIBLE*)
-intros until m2; intros H1 H2 H3.
-destruct H2 as [m1'' [SEM1 SEM2]].
-exploit INJ1; eauto; intros [f'' [m2'' [H4 [H5 [H6 [H7 [H8 H9]]]]]]].
-exploit (INJ2 ge m1'' m1' f''); eauto.
-assert (GLOB_INCR: meminj_preserves_globals ge f'').
- solve[eapply meminj_preserves_globals_incr; eauto].
-eapply GLOB_INCR; eauto.
-intros [f' [m2' [H10 [H11 [H12 [H13 [H14 H15]]]]]]].
-assert (MEMINJ_COMP: 
- forall f f' m1 m2 m3,
-   Mem.inject f m1 m2 -> Mem.inject f' m2 m3 -> 
-   Mem.inject (compose_meminj f f') m1 m3).
- solve[intros; eapply Mem.inject_compose; eauto].
-assert (TRANS: forall P m m'' m',
-  mem_unchanged_on P m m'' -> 
-  mem_unchanged_on P m'' m' -> 
-  mem_unchanged_on P m m').
- intros; eapply mem_unchanged_on_trans; eauto.
-assert (WEAKEN: forall (P P': block -> Z -> Prop) m m',
-  (forall b ofs, P' b ofs -> P b ofs) -> 
-  mem_unchanged_on P m m' -> 
-  mem_unchanged_on P' m m').
- intros; eapply mem_unchanged_on_weaken; eauto.
-exists f'; exists m2'; split.
-exists m2''; split; auto.
-split; auto.
-split; auto.
-eapply mem_unchanged_unmapped_trans; eauto.
-split; auto.
-apply mem_unchanged_outofreach_trans
- with (m2 := m1'') (m2' := m2'') (f2 := f''); auto.
-intros; eapply VALID1; eauto.
-intros.
-eapply PERM1; eauto.
-split; auto.
-eapply inject_incr_trans; eauto.
-clear - SEM1 SEM2 H4 H10 H8 H9 H14 H15 VALID1 VALID2.
-unfold inject_separated in H9, H15|-*.
-intros until delta; intros H1 H2.
-case_eq (f'' b1).
-intros [b1' ofs1'] H3.
-rewrite (H14 _ _ _ H3) in H2.
-inv H2.
-eapply H9; eauto.
-intros H3.
-specialize (H15 _ _ _ H3 H2).
-destruct H15.
-split; intro.
-apply H.
-eapply VALID1; eauto.
-apply H0.
-eapply VALID1; eauto.
-Qed.
-
-End CompilableTrans.
-
-End CompilableSem.
-
-Record CompilableCoreSem {F V C D} := {
-  coresem:> CoreSemantics (Genv.t F V) C mem D;
-  compilable: CompilableSem.Sig (fun bs m m' => exists ge, exists q, exists q',
-      genv2blocks ge=bs /\ corestep coresem ge q m q' m')
-}.
-
-Implicit Arguments CompilableCoreSem [].
-
-(** * Compilable Extensions *)
-
-Module CompilableExtension. Section CompilableExtension.
+Module CompilabilityInvariant. Section CompilabilityInvariant. 
  Variables
   (F V: Type) (** global environments *)
-  (xT: Type) (** corestates of extended semantics *)
-  (cT: nat -> Type) (** corestates of core semantics *)
-  (D: Type) (** initialization data *)
+  (xS xT: Type) (** corestates of source and target extended semantics *)
+  (cS cT: nat -> Type) (** corestates of source and target core semantics *)
+  (dS dT: Type) (** initialization data *)
   (Z: Type) (** external states *)
   (Zint: Type) (** portion of Z implemented by extension *)
   (Zext: Type) (** portion of Z external to extension *)
-  (esem: CoreSemantics (Genv.t F V) xT mem D) (** extended semantics *)
-  (csem: forall i:nat, option (CompilableCoreSem F V (cT i) D)) (** a set of core semantics *)
-
+  (esemS: CoreSemantics (Genv.t F V) xS mem dS) (** extended source semantics *)
+  (esemT: CoreSemantics (Genv.t F V) xT mem dT) (** extended target semantics *)
+  (csemS: forall i:nat, CoreSemantics (Genv.t F V) (cS i) mem dS) (** a set of core semantics *)
+  (csemT: forall i:nat, CoreSemantics (Genv.t F V) (cT i) mem dT) (** a set of core semantics *)
   (csig: ext_sig mem Z) (** client signature *)
   (esig: ext_sig mem Zext) (** extension signature *)
   (handled: list AST.external_function). (** functions handled by this extension *)
 
-Definition cast_csem: forall i:nat, option (CoreSemantics (Genv.t F V) (cT i) mem D) :=
-  fun i => match csem i with Some CS => Some (coresem CS) | None => None end.
+ Variable (E_S: Extension.Sig cS Zint esemS (fun i:nat => Some (csemS i)) csig esig handled).
+ Variable (E_T: Extension.Sig cT Zint esemT (fun i:nat => Some (csemT i)) csig esig handled).
 
-Record Sig := Make { E:> Extension.Sig cT Zint esem cast_csem csig esig handled }.
+ Variable ge: Genv.t F V.
+ Variable entry_points: list (val*val*signature).
+
+ Import Sim_inj.
+
+ Variable core_simulations: forall i:nat, 
+   Forward_simulation_inject dS dT (csemS i) (csemT i) ge ge entry_points.
+
+ Notation PROJ_CORE := (Extension.proj_core).
+ Infix "\o" := (Extension.zmult) (at level 66, left associativity). 
+ Notation ACTIVE := (Extension.active).
+ Notation RUNNABLE := (Extension.runnable).
+ Notation "'CORE' i 'is' ( CS , c ) 'in' s" := 
+   (csem i = Some CS /\ PROJ_CORE i s = Some c)
+   (at level 66, no associativity, only parsing).
+ Notation core_exists := (Extension.core_exists).
+ Notation active_csem := (Extension.active_csem).
+ Notation active_proj_core := (Extension.active_proj_core).
+ Notation notat_external_handled := (Extension.notat_external_handled).
+ Notation at_external_not_handled := (Extension.at_external_not_handled).
+ Notation ext_upd_at_external := (Extension.ext_upd_at_external).
+ Notation runnable_false := (Extension.runnable_false).
+
+ Variable core_data: Type.
+ Variable core_ord: core_data -> core_data -> Prop.
+ Variable match_states: core_data -> meminj -> xS -> mem -> xT -> mem -> Prop.
+
+ Inductive Sig: Type := Make: forall  
+     (corestep_runnable: forall s1 c1 m1 c1' m1' s1' s2 c2 m2 c2' m2' s2' n,
+       PROJ_CORE E_S (ACTIVE E_S s1) s1 = Some c1 -> 
+       PROJ_CORE E_T (ACTIVE E_S s1) s2 = Some c2 -> 
+       RUNNABLE E_S ge s1=RUNNABLE E_T ge s2 -> 
+       corestep (csemS (ACTIVE E_S s1)) ge c1 m1 c1' m1' -> 
+       corestepN (csemT (ACTIVE E_S s1)) ge n c2 m2 c2' m2' -> 
+       corestep esemS ge s1 m1 s1' m1' -> 
+       corestepN esemT ge n s2 m2 s2' m2' -> 
+       RUNNABLE E_S ge s1'=RUNNABLE E_T ge s2')
+     
+     (extension_diagram: forall s1 m1 s1' m1' s2 c1 c2 m2 ef sig args1 args2 cd j,
+       RUNNABLE E_S ge s1=false -> RUNNABLE E_T ge s2=false -> 
+       PROJ_CORE E_S (ACTIVE E_S s1) s1 = Some c1 -> 
+       PROJ_CORE E_T (ACTIVE E_S s1) s2 = Some c2 -> 
+       at_external (csemS (ACTIVE E_S s1)) c1 = Some (ef, sig, args1) -> 
+       at_external (csemT (ACTIVE E_S s1)) c2 = Some (ef, sig, args2) -> 
+       match_states cd j s1 m1 s2 m2 -> 
+       Mem.inject j m1 m2 -> 
+       Events.meminj_preserves_globals ge j -> 
+       Forall2 (val_inject j) args1 args2 -> 
+       Forall2 Val.has_type args2 (sig_args sig) -> 
+       corestep esemS ge s1 m1 s1' m1' -> 
+       exists s2', exists m2', exists cd', exists j',
+         inject_incr j j' /\
+         Events.inject_separated j j' m1 m2 /\
+         match_states cd' j' s1' m1' s2' m2' /\
+         corestep esemT ge s2 m2 s2' m2')
+     
+     (at_external_match: forall s1 m1 s2 c1 c2 m2 ef sig args1 args2 cd j,
+       ACTIVE E_S s1=ACTIVE E_T s2 -> 
+       RUNNABLE E_S ge s1=RUNNABLE E_T ge s2 -> 
+       PROJ_CORE E_S (ACTIVE E_S s1) s1 = Some c1 -> 
+       PROJ_CORE E_T (ACTIVE E_S s1) s2 = Some c2 -> 
+       at_external esemS s1 = Some (ef, sig, args1) -> 
+       at_external (csemS (ACTIVE E_S s1)) c1 = Some (ef, sig, args1) -> 
+       match_state (core_simulations (ACTIVE E_S s1)) cd j c1 m1 c2 m2 -> 
+       Mem.inject j m1 m2 -> 
+       Events.meminj_preserves_globals ge j -> 
+       Forall2 (val_inject j) args1 args2 -> 
+       Forall2 Val.has_type args2 (sig_args sig) -> 
+       at_external (csemT (ACTIVE E_S s1)) c2 = Some (ef, sig, args2) -> 
+       at_external esemT s2 = Some (ef, sig, args2))
+
+     (after_external_runnable: forall ge s1 m1 s2 m2 retv1 retv2 s1' s2' cd j,
+       RUNNABLE E_S ge s1=RUNNABLE E_T ge s2 -> 
+       match_states cd j s1 m1 s2 m2 -> 
+       after_external esemS retv1 s1 = Some s1' -> 
+       after_external esemT retv2 s2 = Some s2' ->     
+       RUNNABLE E_S ge s1'=RUNNABLE E_T ge s2')
+     
+     (make_initial_core_diagram: forall ge v1 vals1 s1 m1 v2 vals2 m2 j sig,
+       make_initial_core esemS ge v1 vals1 = Some s1 -> 
+       Mem.inject j m1 m2 -> 
+       Forall2 (val_inject j) vals1 vals2 -> 
+       Forall2 Val.has_type vals2 (sig_args sig) -> 
+       exists cd, exists s2, 
+         make_initial_core esemT ge v2 vals2 = Some s2 /\
+         match_states cd j s1 m1 s2 m2)
+     
+     (safely_halted_step: forall cd j c1 m1 c2 m2 ge v1,
+       match_states cd j c1 m1 c2 m2 -> 
+       safely_halted esemS ge c1 = Some v1 -> 
+       exists v2,
+         val_inject j v1 v2 /\
+         safely_halted esemT ge c2 = Some v2 /\ 
+         Mem.inject j m1 m2)
+     
+     (safely_halted_diagram: forall cd j m1 m1' m2 rv s1 s2 s1' c1 c2,
+       match_states cd j s1 m1 s2 m2 -> 
+       PROJ_CORE E_S (ACTIVE E_S s1) s1 = Some c1 -> 
+       PROJ_CORE E_T (ACTIVE E_S s1) s2 = Some c2 -> 
+       safely_halted (csemS (ACTIVE E_S s1)) ge c1 = Some rv -> 
+       corestep esemS ge s1 m1 s1' m1' ->  
+       safely_halted (csemT (ACTIVE E_S s1)) ge c2 = Some rv /\
+       exists s2', exists m2', exists cd', exists j', 
+         inject_incr j j' /\
+         Events.inject_separated j j' m1 m2 /\
+         corestep esemT ge s2 m2 s2' m2' /\
+         match_states cd' j' s1' m1' s2' m2'),
+     Sig.
+
+End CompilabilityInvariant. End CompilabilityInvariant.
+
+Module CompilableExtension. Section CompilableExtension. 
+ Variables
+  (F V: Type) (** global environments *)
+  (xS xT: Type) (** corestates of source and target extended semantics *)
+  (cS cT: nat -> Type) (** corestates of source and target core semantics *)
+  (dS dT: Type) (** initialization data *)
+  (Z: Type) (** external states *)
+  (Zint: Type) (** portion of Z implemented by extension *)
+  (Zext: Type) (** portion of Z external to extension *)
+  (esemS: CoreSemantics (Genv.t F V) xS mem dS) (** extended source semantics *)
+  (esemT: CoreSemantics (Genv.t F V) xT mem dT) (** extended target semantics *)
+  (csemS: forall i:nat, CoreSemantics (Genv.t F V) (cS i) mem dS) (** a set of core semantics *)
+  (csemT: forall i:nat, CoreSemantics (Genv.t F V) (cT i) mem dT) (** a set of core semantics *)
+  (csig: ext_sig mem Z) (** client signature *)
+  (esig: ext_sig mem Zext) (** extension signature *)
+  (handled: list AST.external_function). (** functions handled by this extension *)
+
+ Variable (E_S: Extension.Sig cS Zint esemS (fun i:nat => Some (csemS i)) csig esig handled).
+ Variable (E_T: Extension.Sig cT Zint esemT (fun i:nat => Some (csemT i)) csig esig handled).
+
+ Variable ge: Genv.t F V.
+ Variable entry_points: list (val*val*signature).
+
+ Import Sim_inj.
+
+ Variable core_simulations: forall i:nat, 
+   Forward_simulation_inject dS dT (csemS i) (csemT i) ge ge entry_points.
+
+ Record Sig: Type := Make {
+   core_data: Type;
+   core_ord: core_data -> core_data -> Prop;
+   match_states: core_data -> meminj -> xS -> mem -> xT -> mem -> Prop;
+   _ : (forall i: nat, RelyGuaranteeSimulation.Sig (core_simulations i)) -> 
+       CompilabilityInvariant.Sig csemS csemT E_S E_T core_simulations match_states -> 
+       Forward_simulation_inject dS dT esemS esemT ge ge entry_points
+ }.
 
 End CompilableExtension. End CompilableExtension.
-  
